execution/examples/Congress_Buggy.v
@@ -318,7 +318,7 @@ Section Theories.
                block_finalized_height := finalized_height chain;
                block_creator := creator;
                block_reward := 50; |} in
-        let acts := map (build_act creator eq_refl creator) act_bodies in
+        let acts := map (build_act creator creator) act_bodies in
         option_of_result (builder_add_block chain next_header acts) in
     (* Get some money on the creator *)
     do chain <- add_block chain [];
