execution/examples/Dexter2FA12.v
@@ -971,12 +971,11 @@ Proof.
     destruct_action_eval; auto.
 Qed.
 
-Lemma no_self_calls' : forall bstate origin origin_valid from_addr to_addr amount msg acts,
+Lemma no_self_calls' : forall bstate origin from_addr to_addr amount msg acts,
   reachable bstate ->
   env_contracts bstate to_addr = Some (contract : WeakContract) ->
   chain_state_queue bstate =
   {| act_origin := origin;
-     act_origin_valid := origin_valid;
      act_from := from_addr;
      act_body :=
        match msg with
@@ -1073,10 +1072,7 @@ Proof.
     subst. cbn.
     split.
     + now apply Z.ge_le.
-    + match goal with
-      | [H : act = _ |- _] => rewrite H in *
-      end.
-      now eapply no_self_calls'.
+    + now eapply no_self_calls'.
 Qed.
 
 Lemma contract_balance_bound : forall bstate caddr (trace : ChainTrace empty_state bstate),
