execution/tests/EscrowTests/EscrowGens.v
@@ -32,10 +32,9 @@ Definition gAccountWithBalance (e : Env) (gAccOpt : GOpt Address) : GOpt (Addres
   returnGenSome (addr, e.(env_account_balances) addr).
 
 Definition gEscrowMsg (e : Env) : GOpt Action :=
-  let call caller caller_is_user amount msg :=
+  let call caller amount msg :=
       returnGenSome {|
           act_origin := caller;
-          act_origin_valid := caller_is_user;
           act_from := caller;
           act_body := act_call contract_addr amount (@serialize Escrow.Msg _ msg)
         |} in
@@ -51,16 +50,13 @@ Definition gEscrowMsg (e : Env) : GOpt Action :=
         if e.(env_account_balances) buyer <? 2
         then returnGen None
         else
-          p <- validate_origin buyer ;;
-          call buyer p 2 commit_money
+          call buyer 2 commit_money
     ) ;
     (* confirm received item *)
-    (1%nat, p <- validate_origin buyer ;;
-          call buyer p 0 confirm_item_received) ;
+    (1%nat, call buyer 0 confirm_item_received) ;
     (* withdraw money *)
     (1%nat, addr <- elems [seller; buyer] ;;
-            p <- validate_origin addr ;;
-            call addr p 0 withdraw
+            call addr 0 withdraw
     )
   ].
 
@@ -69,10 +65,9 @@ Definition gEscrowMsg (e : Env) : GOpt Action :=
    This should lead to much fewer discards during testing, but at the cost of the generator being more complex
    and less "blackbox-like" *)
 Definition gEscrowMsgBetter (e : Env) : GOpt Action :=
-  let call caller caller_is_user amount msg :=
+  let call caller amount msg :=
       returnGenSome {|
           act_origin := caller;
-          act_origin_valid := caller_is_user;
           act_from := caller;
           act_body := act_call contract_addr amount (@serialize Escrow.Msg _ msg)
   |} in
@@ -85,24 +80,18 @@ Definition gEscrowMsgBetter (e : Env) : GOpt Action :=
                       (2%nat, if e.(env_account_balances) buyer <? 2
                               then returnGen None
                               else
-                                p <- validate_origin buyer ;;
-                                call buyer p 2 commit_money
+                                call buyer 2 commit_money
                       );
                      (1%nat,
-                      p <- validate_origin seller ;;
-                      call seller p 0 withdraw)
+                      call seller 0 withdraw)
                     ]
-  | buyer_confirm =>
-    p <- validate_origin buyer ;;
-    call buyer p 0 confirm_item_received
+  | buyer_confirm => call buyer 0 confirm_item_received
   | _ => if 0 <? state.(buyer_withdrawable)
         then
-          p <- validate_origin buyer ;;
-          call buyer p 0 withdraw
+          call buyer 0 withdraw
          else if 0 <? state.(seller_withdrawable)
               then
-                p <- validate_origin seller ;;
-                call seller p 0 withdraw
+                call seller 0 withdraw
          else returnGen None
   end.
 
